certicoq/theories/L1_MalechaQuoted/wNorm.v
@@ -113,43 +113,50 @@ Lemma Wcbv_WNorm:
     (forall ts ss, WcbvEvals p ts ss -> WFapps ts -> WNorms ss) /\
     (forall dts dss, WcbvDEvals p dts dss ->  WFappDs dts -> WDNorms dss).
 Proof.
-intros hp. apply WcbvEvalEvals_ind; simpl; intros; auto.
-- inversion_Clear H0. intuition. 
-- inversion_Clear H0. intuition. 
-- inversion_Clear H1. apply H. assumption.
-- constructor. apply H. inversion H0. assumption.
-- inversion_Clear H0. apply H.
-  assert (j:= Lookup_pres_WFapp hp l). inversion j. assumption.
+  intros hp.
+  apply WcbvEvalEvals_ind; simpl; intros; try (solve[constructor]);
+  try inversion_Clear H0; intuition.
+  - apply H. assert (j:= Lookup_pres_WFapp hp l). inversion j. assumption.
 - inversion_Clear H2. apply H1. 
   assert (j:= proj1 (wcbvEval_pres_WFapp hp) _ _ w H7). inversion_Clear j.
   apply whBetaStep_pres_WFapp; try assumption.
-  eapply (proj1 (wcbvEval_pres_WFapp hp)); eassumption. 
-- inversion_Clear H2. apply H1. apply instantiate_pres_WFapp. assumption. 
-  apply (proj1 (wcbvEval_pres_WFapp hp) _ _ w). assumption.
-- apply H0. inversion_Clear H1.
+  eapply (proj1 (wcbvEval_pres_WFapp hp)); eassumption.
+- inversion_Clear H1. apply H0. apply instantiate_pres_WFapp.
+  + assumption.
+  + refine (proj1 (wcbvEval_pres_WFapp hp) _ _ _ _); eassumption.
+ - apply H0. inversion_Clear H1.
   refine (whFixStep_pres_WFapp _ _ _). 
   + assert (j:= proj1 (wcbvEval_pres_WFapp hp) _ _ w H6).
     inversion j. assumption.
-  + constructor; assumption.
+  + constructor; intuition.
 - inversion_Clear H2.
   constructor; intuition; unfold isLambda, isFix, isApp in *.
   + destruct H2 as [x1 [x2 [x3 j]]]. discriminate.
   + destruct H2 as [x1 [x2 j]]. discriminate.
   + destruct H2 as [x1 [x2 [x3 j]]]. discriminate.
-- apply H1. refine (whCaseStep_pres_WFapp _ _ _ e); try constructor.
-  inversion H2. assumption.
-- inversion_Clear H2. apply H1. refine (whCaseStep_pres_WFapp _ _ _ e0).
+- inversion_Clear H2.
+  constructor; intuition; unfold isLambda, isFix, isApp in *.
+  + destruct H2 as [x1 [x2 [x3 j]]]. discriminate.
+  + destruct H2 as [x1 [x2 j]]. discriminate.
+  + destruct H2 as [x1 [x2 [x3 j]]]. discriminate.
+- inversion_Clear H2.
+  constructor; intuition; unfold isLambda, isFix, isApp in *.
+  + destruct H2 as [x1 [x2 [x3 j]]]. discriminate.
+  + destruct H2 as [x1 [x2 j]]. discriminate.
+  + destruct H2 as [x1 [x2 [x3 j]]]. discriminate.
+- inversion_Clear H1. apply H0. refine (whCaseStep_pres_WFapp _ _ _ e).
+  + assumption.
+  + constructor.
+- inversion_Clear H1. apply H0. refine (whCaseStep_pres_WFapp _ _ _ e0).
   + assumption.
   + refine (tskipn_pres_WFapp _ _ e).
-    assert (j:= proj1 (wcbvEval_pres_WFapp hp) _ _ w H6). inversion_Clear j.
+    assert (j:= proj1 (wcbvEval_pres_WFapp hp) _ _ w H5). inversion_Clear j.
     constructor; assumption.
 - inversion_Clear H2. constructor; try (solve[intuition]).
   intros h. inversion h.
-- constructor. 
 - inversion_Clear H1. constructor; intuition.
 - inversion_Clear H2. constructor; intuition.
 Qed.
-
 
 Lemma wcbvEval_no_further:
     (forall t s, WcbvEval p t s -> WcbvEval p s s) /\
